(with @R1kM) WIP server_ClientHello

src/tls/Test.TLS.Send.fst
@@ -35,18 +35,18 @@ noeq type handshake = | HS:
 //  state: ref machineState {HS.frameOf state = region} -> // state machine; should be opaque and depend on r.
   handshake
 
-let valid (hs:handshake) (h:HS.mem) =
+let invariant (hs:handshake) (h:HS.mem) =
   TS.invariant hs.sto h /\
   T.invariant hs.stt (Ghost.reveal hs.t) h /\
-  h `HS.contains` hs.nego.Nego.state /\
+  Nego.inv hs.nego h /\
   B.loc_disjoint (TS.footprint hs.sto) (T.footprint hs.stt) /\
-  B.loc_disjoint (TS.footprint hs.sto) (B.loc_mreference hs.nego.Nego.state) /\
-  B.loc_disjoint (T.footprint hs.stt) (B.loc_mreference hs.nego.Nego.state)
+  B.loc_disjoint (TS.footprint hs.sto) (Nego.footprint hs.nego) /\
+  B.loc_disjoint (T.footprint hs.stt) (Nego.footprint hs.nego)
 
 let footprint (hs:handshake) =
   TS.footprint hs.sto `B.loc_union`
   T.footprint hs.stt `B.loc_union` 
-  B.loc_mreference hs.nego.Nego.state
+  Nego.footprint hs.nego
 
 let is_state13 (hs:handshake) = T.Transcript13? (Ghost.reveal hs.t)
 
@@ -60,14 +60,14 @@ assume val signature:HSM13.handshake13_m13_certificate_verify
 // TODO: should tag be allocated inside of a function? on the stack?
 
 val serverFinished: hs:handshake -> tag:Hacl.Hash.Definitions.hash_t (hs.a) -> ST (result handshake)
-    (requires fun h -> valid hs h /\ B.live h tag /\ is_state13 hs /\
+    (requires fun h -> invariant hs h /\ B.live h tag /\ is_state13 hs /\
       Ghost.reveal hs.n < T.max_transcript_size - 4 /\
       B.loc_disjoint (B.loc_buffer tag) (B.loc_region_only true Mem.tls_tables_region) /\
       B.loc_disjoint (B.loc_buffer tag) (footprint hs))
     (ensures fun h0 res h1 -> 
       B.(modifies (footprint hs `loc_union` loc_buffer tag `loc_union` loc_region_only true Mem.tls_tables_region)) h0 h1 /\
       begin match res with
-      | Correct hs' -> valid hs' h1
+      | Correct hs' -> invariant hs' h1
       | _ -> True
       end
     )
@@ -126,3 +126,152 @@ let serverFinished hs tag =
       | Error z -> Error z
       end
     | Error z -> Error z
+
+
+val server_ClientHello: 
+  #region: _ -> ns: Nego.t region TLSConstants.Server ->
+  out: TS.send_state ->
+  T.hs_ch -> 
+  ST (result handshake)
+  (requires fun h0 -> 
+    Mem.is_hs_rgn region /\
+    Nego.inv ns h0 /\
+    TS.invariant out h0 /\
+    B.loc_disjoint (TS.footprint out) (Nego.footprint ns) /\
+    (let s = HS.sel h0 ns.Nego.state in Nego.S_Init? s)) // TODO:  \/ Nego.S_HRR? s
+  (ensures fun h0 r h1 -> 
+    B.modifies (Nego.footprint ns `B.loc_union` TS.footprint out `B.loc_union` B.loc_region_only true Mem.tls_tables_region) h0 h1 /\
+    begin match r with
+    | Correct hs ->
+      invariant hs h1 /\
+      hs.region == region /\
+      hs.r == TLSConstants.Server /\
+      hs.nego == ns /\
+      T.ClientHello? (Ghost.reveal hs.t)
+      // TODO: /\ hs.t == ...
+    |  _ -> True
+    end
+    )
+  // [S_Init | S_HRR ==> S_ClientHello m cert] 
+  // ensures r = computeServerMode ns.cfg ns.nonce offer (stateful)
+  // but [compute_cs13] and [negotiateCipherSuite] are pure. 
+
+assume val computeServerMode: result Nego.serverMode
+
+assume val find_cookie: Nego.offer -> option Extensions.cookie 
+
+assume val serverMode_hashAlg: Nego.serverMode -> Tot Hashing.Spec.alg
+
+(*
+  cfg: TLSConstants.config ->
+  co: TLSConstants.offer ->
+  serverRandom: TLSInfo.random ->
+  ST (result serverMode)
+  (requires fun h0 -> True)
+  (ensures fun h0 r h1 -> 
+    B.(modifies loc_none h0 h1) /\ 
+    ( match r with 
+      | Correct (ServerRetry hrr) -> TLS.Cookie.hrr_len hrr <= 16 // leaving enough room for the cookie 
+      | _ -> True )
+    )
+*)
+
+#push-options "--z3rlimit 300 --max_ifuel 8 --initial_ifuel 8"
+
+let server_ClientHello #region ns out offer =
+// TODO: match !ns.Nego.state with  | Nego.S_HRR o1 hrr -> server_ClientHello2_stateful ns o1 hrr offer
+//  | Nego.S_Init _ ->
+    let sm = computeServerMode in // ns.Nego.cfg offer ns.Nego.nonce in
+    match sm with
+    | Error z -> Error z
+    | Correct r ->
+      let h = get() in
+      // TRANSCRIPT:
+      let tr = T.create region (serverMode_hashAlg r) in
+      let stateless_retry = 
+        match find_cookie (HSM.M_client_hello?._0 offer) with
+        | None -> None 
+        | Some c ->
+          // stateless HRR.
+          match TLS.Cookie.decrypt c with
+          | Error _ -> 
+            // This connection is doomed: we could instead return a fatal error. 
+            None
+            
+          | Correct (digest, extra, hrr) ->
+            // TODO check consistency of sm with hrr's cs and group;
+            // this is required to enforce the earlier server policy.
+
+            // Lowering: we can use the output buffer as scratch space
+            // for outputting the digest (of known size) and the hrr
+            // (possibly quite large), since we only need them for
+            // computing the transcript digest.
+            //
+            // Alternatively, we could pass the hrr in two chunks: the
+            // (small, reconstructed) hrr prefix, and the (received)
+            // encrypted cookie.
+            //
+            // TRANSCRIPT 
+            // extend_stateless hrr digest hrr //{ Start(None) --HRR digest hrr--> Start(Some(digest,hrr)) }
+            // using sm's hash algorithm. 
+            Some extra // to be passed to the server nego callback
+        in 
+        fatal Handshake_failure "negotiation failed after a retry"
+      
+(*
+
+      // let tr = Transcript.create (ha_of_sm sm) in // { state(tr) == Start(None) }
+      
+
+      // TRANSCRIPT 
+      // extend_ch offer //{ Start(r) --> ClientHello(r,offer) }
+      let h = get() in assert (inv ns h);
+      match r with 
+      | ServerRetry hrr -> (
+        if Some? stateless_retry then 
+          fatal Handshake_failure "negotiation failed after a retry"
+        else (
+          // Internal HRR caused by group negotiation
+          // We do not invoke the server nego callback in this case
+          // record the initial offer and return the HRR to HS
+          trace ("no common group, sending a retry request...");
+          // TODO create Transcript in state Start(Some(digest,hrr)) to compute this digest
+          let ha = TLS.Cookie.hrr_ha hrr in 
+          let digest = HandshakeLog.hash_tag #ha log0 in 
+          let hrr = TLS.Cookie.append digest empty_bytes hrr in
+          ns.state := S_HRR offer hrr;
+          sm ))
+
+      | ServerMode m cert _ -> (
+        let nego_cb = ns.cfg.nego_callback in
+        let exts = List.Tot.filter CHE_Unknown_extensionType? offer.CH.extensions in
+        // 19-06-16 recurring problem with list filtering; might disappear by lowering, or we could use the list serializer.
+        assume(clientHelloExtensions_list_bytesize exts <= 65535);
+        let exts_bytes = clientHelloExtensions_serializer32 exts in
+        trace ("Negotiation callback to handle extra extensions and query for stateless retry.");
+        trace ("Application data in cookie: "^(match stateless_retry with | Some c -> hex_of_bytes c | _ -> "none"));
+        let r = nego_cb.negotiate nego_cb.nego_context m.n_protocol_version exts_bytes stateless_retry in
+        let h = get() in assert (inv ns h);
+        match r with 
+        | Nego_abort -> (
+          trace ("Application requested to abort the handshake.");
+          fatal Handshake_failure "application requested to abort the handshake.")
+
+        | Nego_retry filling -> (
+          trace ("Application requested to retry the handshake.");
+          assume(CipherSuite13? m.n_cipher_suite); // from ServerMode 
+          let hrr = TLS.Cookie.hrr0 offer.CH.session_id m.n_cipher_suite in
+          let ha = TLS.Cookie.hrr_ha hrr in 
+          let digest = HandshakeLog.hash_tag #ha log0 in
+          let hrr = TLS.Cookie.append digest filling hrr in
+          ns.state := S_HRR offer hrr;
+          Correct (ServerRetry hrr))
+        
+        | Nego_accept sexts -> (
+          trace ("Application accepted "^
+            string_of_pv m.n_protocol_version^" "^
+            string_of_ciphersuite m.n_cipher_suite);
+          ns.state := S_ClientHello m cert;
+          Correct (ServerMode m cert sexts)))) in
+  r
+#pop-options
